Compiles -- without CompilerC

demo/mutrec/SimMemInjInvC.v
@@ -10,10 +10,7 @@ Require Import IntegersC LinkingC.
 Require Import SimSymb Skeleton Mod ModSem.
 Require Import SimMem.
 Require SimSymbId.
-Require Import Conventions1.
-Require MachC.
-Require Export SimMemInj.
-Require Import SimMemInjC.
+Require Export SimMemInjInv.
 Require Import Coq.Logic.FunctionalExtensionality.
 Require Import Coq.Logic.ClassicalChoice.
 Require Import Coq.Logic.ChoiceFacts.
@@ -24,129 +21,14 @@ Set Implicit Arguments.
 
 Section MEMINJINV.
 
-  Definition memblk_invariant := (memory_chunk -> Z -> option val) -> Prop.
-  (* Definition memory_invariant := block -> memblk_invariant -> Prop. *)
-
   Variable P : memblk_invariant.
 
-  (* Record t' := mk *)
-  (*   { minj:> SimMemInj.t'; *)
-  (*     src_genv_nb : block; *)
-  (*     tgt_genv_nb : block; *)
-  (*     mem_inv: block -> Prop; *)
-  (*     (* mem_inv: block -> (memory_chunk -> Z -> option val -> Prop); *) *)
-  (*   }. *)
-
-  Record t' :=
-    mk
-      { src : mem;
-        tgt : mem;
-        inj : meminj;
-        mem_inv: block -> Prop;
-        (* mem_inv: memory_invariant; *)
-      }.
-
-  (* Definition tgt_private_nge (sm: t') := *)
-  (*   (loc_out_of_reach sm.(inj) sm.(src)) *)
-  (*     /2\ (valid_blocks sm.(tgt)) /2\ (fun blk _ => Ple blk sm.(tgt_genv_nb)). *)
-
-  (* Definition src_private_nge (sm: t') := *)
-  (*   (loc_unmapped sm.(inj)) *)
-  (*     /2\ (valid_blocks sm.(src)) /2\ (fun blk _ => Ple blk sm.(src_genv_nb)). *)
-
-  Definition inv_sat_blk blk (invar: memblk_invariant) (m: mem): Prop :=
-    invar (fun chunk ofs =>
-             if (Mem.valid_access_dec m chunk blk ofs Writable)
-             then Mem.load chunk m blk ofs
-             else None).
-
-  (* Definition inv_sat_mem (invar: memory_invariant) (m: mem) : Prop := *)
-  (*   forall blk inv_blk (INVAR: invar blk inv_blk), inv_sat_blk blk inv_blk m.   *)
-
-  Definition inv_sat_mem (invar: block -> Prop) (m: mem) : Prop :=
-    forall blk (INVAR: invar blk), inv_sat_blk blk P m.
-
-  Inductive wf' (sm0: t'): Prop :=
-  | wf_intro
-      (WF: Mem.inject sm0.(inj) sm0.(src) sm0.(tgt))
-      (SAT: inv_sat_mem sm0.(mem_inv) sm0.(tgt))
-      (INVRANGE: forall blk ofs (INV: sm0.(mem_inv) blk),
-          loc_out_of_reach sm0.(inj) sm0.(src) blk ofs /\ Mem.valid_block sm0.(tgt) blk)
-      (* (INVRANGE: forall blk ofs invar (INV: sm0.(mem_inv) blk invar),         *)
-      (*     loc_out_of_reach sm0.(inj) sm0.(src) blk ofs /\ Mem.valid_block sm0.(tgt) blk) *)
-  .
-
-  Lemma unchanged_on_invariant invar m0 m1
-        (INVAR: inv_sat_mem invar m0)
-        (INVRANGE: invar <1= Mem.valid_block m0)
-        (UNCH: Mem.unchanged_on (fun blk _ => invar blk) m0 m1)
-    :
-      inv_sat_mem invar m1.
-  Proof.
-    ii. exploit INVAR; eauto. intros SAT.
-    unfold inv_sat_blk in *. rp; eauto.
-    extensionality chunk. extensionality ofs.
-    des_ifs.
-    - eapply Mem.load_unchanged_on_1; eauto.
-    - exfalso. apply n. inv v. split; auto.
-      ii. eapply Mem.perm_unchanged_on_2; eauto.
-    - exfalso. apply n. inv v. split; auto.
-      ii. eapply Mem.perm_unchanged_on; eauto.
-  Qed.
-
-  Inductive le' (mrel0 mrel1: t'): Prop :=
-  | le_intro
-      (SRCNBLE: Ple mrel0.(src).(Mem.nextblock) mrel1.(src).(Mem.nextblock))
-      (TGTNBLE: Ple mrel0.(tgt).(Mem.nextblock) mrel1.(tgt).(Mem.nextblock))
-      (INCR: inject_incr mrel0.(inj) mrel1.(inj))
-      (FROZEN: inject_separated
-                 (mrel0.(inj)) (mrel1.(inj))
-                 (mrel0.(src)) (mrel0.(tgt)))
-      (MINVEQ: mrel0.(mem_inv) = mrel1.(mem_inv))
-      (MAXSRC: forall
-          b ofs
-          (VALID: Mem.valid_block mrel0.(src) b)
-        ,
-          <<MAX: Mem.perm mrel1.(src) b ofs Max <1= Mem.perm mrel0.(src) b ofs Max>>)
-      (MAXTGT: forall
-          b ofs
-          (VALID: Mem.valid_block mrel0.(tgt) b)
-        ,
-          <<MAX: Mem.perm mrel1.(tgt) b ofs Max <1= Mem.perm mrel0.(tgt) b ofs Max>>)
-  .
-
-  Global Program Instance le'_PreOrder: RelationClasses.PreOrder le'.
-  Next Obligation.
-    econs; ss; eauto.
-    - refl.
-    - refl.
-    - ii. clarify.
-  Qed.
-  Next Obligation.
-    ii. inv H. inv H0. econs; eauto.
-    - etrans; eauto.
-    - etrans; eauto.
-    - etrans; eauto.
-    - ii. destruct (inj y b1) as [[b3 delta0]|] eqn:DELTA.
-      + dup DELTA. eapply INCR0 in DELTA. clarify.
-        exploit FROZEN; eauto.
-      + dup DELTA. exploit FROZEN0; eauto. i. des.
-        unfold Mem.valid_block in *. split; ii.
-        * eapply H1. eapply Plt_Ple_trans; eauto.
-        * eapply H2. eapply Plt_Ple_trans; eauto.
-    - etrans; eauto.
-    - ii. eapply MAXSRC; eauto. eapply MAXSRC0; eauto.
-      eapply Plt_Ple_trans; eauto.
-    - ii. eapply MAXTGT; eauto. eapply MAXTGT0; eauto.
-      eapply Plt_Ple_trans; eauto.
-  Qed.
-  
   Global Program Instance SimMemInjInv : SimMem.class :=
     {
       t := t';
       src := src;
       tgt := tgt;
-      wf := wf';
+      wf := wf' P;
       le := le';
       lift := fun sm => sm;
       unlift := fun _ sm => sm;
@@ -174,52 +56,6 @@ Section MEMINJINV.
     inv MLE. rewrite MINVEQ. auto.
   Qed.
 
-  Lemma unchanged_on_mle sm0 m_src1 m_tgt1 j1
-        (WF: wf' sm0)
-        (INJECT: Mem.inject j1 m_src1 m_tgt1)
-        (INCR: inject_incr sm0.(inj) j1)
-        (SEP: inject_separated sm0.(inj) j1 sm0.(src) sm0.(tgt))
-        (UNCHSRC: Mem.unchanged_on
-                    (loc_unmapped sm0.(inj))
-                    sm0.(src) m_src1)
-        (UNCHTGT: Mem.unchanged_on
-                    (loc_out_of_reach sm0.(inj) sm0.(src))
-                    sm0.(tgt) m_tgt1)
-        (MAXSRC: forall
-            b ofs
-            (VALID: Mem.valid_block sm0.(src) b)
-          ,
-            <<MAX: Mem.perm m_src1 b ofs Max <1= Mem.perm sm0.(src) b ofs Max>>)
-        (MAXTGT: forall
-            b ofs
-            (VALID: Mem.valid_block sm0.(tgt) b)
-          ,
-            <<MAX: Mem.perm m_tgt1 b ofs Max <1= Mem.perm sm0.(tgt) b ofs Max>>)
-    :
-      (<<MLE: le' sm0 (mk m_src1 m_tgt1 j1 sm0.(mem_inv))>>) /\
-      (<<MWF: wf' (mk m_src1 m_tgt1 j1 sm0.(mem_inv))>>).
-  Proof.               
-    split.
-    - econs; ss; eauto.
-      + eapply Mem.unchanged_on_nextblock; eauto.
-      + eapply Mem.unchanged_on_nextblock; eauto.
-    - inv WF. econs; ss; eauto.
-      + eapply unchanged_on_invariant; eauto.
-        * ii. eapply INVRANGE; eauto. apply 0.
-        * eapply Mem.unchanged_on_implies; eauto.
-          i. eapply INVRANGE; eauto.
-      + i. exploit INVRANGE; eauto. i. des. split.
-        * ii. destruct (inj sm0 b0) as [[blk0 delta0]|] eqn:DELTA.
-          { dup DELTA. apply INCR in DELTA. clarify.
-            eapply INVRANGE; eauto. eapply MAXSRC; eauto.
-            eapply Mem.valid_block_inject_1; eauto. }
-          { exploit SEP; eauto. i. des. clarify. }
-        * eapply Plt_Ple_trans; eauto.
-          eapply Mem.unchanged_on_nextblock; eauto.
-
-          Unshelve. apply 0.
-  Qed.          
-  
 End MEMINJINV.
 
 
@@ -582,6 +418,7 @@ Section SIMSYMBINV.
   Next Obligation.
     inv MLE. inv SIMSKENV. inv SIMSKENV0.
     destruct sm0, sm1. ss. clarify.
+    rename inj0 into inj1. rename inj into inj0.
     econs; ss; eauto.
     - inv INJECT. econs; ss; eauto.
       + i. destruct (inj1 b) as [[b0 delta]|]eqn:BLK; auto.
