backend/UnreadglobproofC.v
@@ -1,0 +1,389 @@
+Require Import FSets CoqlibC Maps Ordered Iteration Errors.
+Require Import AST Linking.
+Require Import IntegersC ValuesC Memory Globalenvs Events Smallstep.
+Require Import Op Registers RTLC.
+Require Import Unreadglob.
+Require Import sflib.
+Require SimMemInjInv.
+(** newly added **)
+Require Export Unreadglobproof.
+Require Import Simulation.
+Require Import Skeleton Mod ModSem SimMod SimModSem SimSymb SimMem AsmregsC MatchSimModSem.
+Require SimMemInjInvC.
+Require SimSymbDropInv.
+Require SoundTop.
+Require Import CtypingC.
+Require Import ModSemProps.
+Require Import JunkBlock.
+
+Set Implicit Arguments.
+
+
+
+Let SM := SimMemInjInvC.SimMemInjInv top1.
+Local Existing Instance SM.
+
+Section SIMMODSEM.
+
+Variable skenv_link_src skenv_link_tgt: SkEnv.t.
+Variable sm_link: SimMem.t.
+Variable prog: RTL.program.
+Variable tprog: RTL.program.
+Let md_src: Mod.t := (RTLC.module prog).
+Let md_tgt: Mod.t := (RTLC.module tprog).
+Hypothesis (INCLSRC: SkEnv.includes skenv_link_src md_src.(Mod.sk)).
+Hypothesis (INCLTGT: SkEnv.includes skenv_link_tgt md_tgt.(Mod.sk)).
+Hypothesis (WFSRC: SkEnv.wf skenv_link_src).
+Hypothesis (WFTGT: SkEnv.wf skenv_link_tgt).
+Hypothesis TRANSL: match_prog prog tprog.
+Let ge := (SkEnv.revive (SkEnv.project skenv_link_src md_src.(Mod.sk)) prog).
+Let tge := (SkEnv.revive (SkEnv.project skenv_link_tgt md_tgt.(Mod.sk)) tprog).
+Definition msp: ModSemPair.t :=
+  ModSemPair.mk (md_src.(Mod.modsem) skenv_link_src) (md_tgt.(Mod.modsem) skenv_link_tgt)
+                ((prog.(defs) -1 tprog.(defs) -1 (Pos.eq_dec tprog.(prog_main))): ident -> Prop)
+                sm_link
+.
+
+Inductive match_states
+          (sm_init: SimMem.t)
+          (idx: nat) (st_src0: RTL.state) (st_tgt0: RTL.state) (sm0: SimMem.t): Prop :=
+| match_states_intro
+    (MATCHST: Unreadglobproof.match_states prog tprog (used_set tprog) skenv_link_src skenv_link_tgt ge tge st_src0 st_tgt0 sm0)
+    (MCOMPATSRC: st_src0.(RTL.get_mem) = sm0.(SimMem.src))
+    (MCOMPATTGT: st_tgt0.(RTL.get_mem) = sm0.(SimMem.tgt))
+.
+
+Lemma find_funct_inject
+      used fptr tfptr fd j
+      (SIMGE: meminj_preserves_globals prog tprog used ge tge j)
+      (FINDSRC: Genv.find_funct ge fptr = Some fd)
+      (INJ: Val.inject j fptr tfptr)
+  :
+    <<FINDTGT: Genv.find_funct tge tfptr = Some (transf_fundef (transf_function (fun _ i => filter_instr used i)) fd)>>
+.
+Proof.
+  inv SIMGE.
+  uge0. des_ifs_safe.
+  inv INJ.
+  exploit defs_inject; et. i; des. clarify. psimpl. des_ifs.
+Qed.
+
+Theorem sim_skenv_meminj_preserves_globals
+        sm_arg
+        (SIMSKENV:
+           SimSymbDropInv.sim_skenv
+             sm_arg ((prog.(defs) -1 tprog.(defs) -1 (Pos.eq_dec tprog.(prog_main))): ident -> Prop)
+             (SkEnv.project skenv_link_src md_src.(Mod.sk)) (SkEnv.project skenv_link_tgt md_tgt.(Mod.sk)))
+  :
+    <<SIMGE: meminj_preserves_globals prog tprog (used_set tprog) ge tge (SimMemInjInv.inj sm_arg)>>
+.
+Proof.
+  exploit SkEnv.project_revive_precise; et.
+  { eapply SkEnv.project_impl_spec; et. eapply INCLSRC. }
+  { ss. }
+  intro GESRC.
+
+  inv SIMSKENV. ss. bar.
+  destruct TRANSL as [used0 TRANSL0]. desH TRANSL0. clarify.
+  econs.
+  - i. exploit SIMSYMB1; et. i; des. clarify. esplits; eauto.
+    unfold used_set. des_sumbool. ss. apply not_and_or in KEPT. des; eauto.
+    + apply not_and_or in KEPT. des; eauto.
+      { exfalso. apply KEPT. inv GESRC. exploit SYMB2P; eauto. }
+      { right. apply NNPP in KEPT. unfold defs in KEPT. des_sumbool. ss. }
+    + left. apply NNPP in KEPT. des_sumbool. ss.
+  - i. exploit SIMSYMB2; et.
+    { ii. des. unfold used_set in *. ss. des_sumbool.
+      align_bool; bsimpl. des_sumbool.
+      des; clarify.
+      unfold defs in *. des_sumbool. ss.
+    }
+  - eauto.
+  - i. unfold ge in H0. exploit Genv_map_defs_def; et. i; des.
+    exploit SIMDEF; et. i; des. clarify. psimpl.
+    uo. des_ifs_safe.
+    exploit Genv.invert_find_symbol; et. intro SYMBSRC; des.
+    exploit SIMSYMB1; et. i; des. psimpl. clear_tac. 
+    exploit Genv.find_invert_symbol; et. intro SYMBTGT; des.
+
+    destruct (classic (defs prog i)); cycle 1.
+    { clear - Heq1 H1. contradict H1. unfold defs in *. des_sumbool. apply prog_defmap_spec; et. }
+    assert(KEPT0: (defs tprog i \/ Pos.eq_dec (prog_main tprog) i)).
+    { tauto. }
+    clear KEPT.
+    assert(IN: (used_set tprog) i).
+    { clarify. unfold used_set. des_sumbool. ss. des; des_sumbool; eauto. right.
+      unfold defs in KEPT0. des_sumbool. ss.
+    }
+
+    esplits; et.
+    + unfold tge.
+      unfold SkEnv.revive.
+      erewrite Genv_map_defs_def_inv; et.
+      uo. des_ifs_safe.
+      erewrite match_prog_def; et. rewrite Heq1. ss. des_ifs_safe.
+      (* exploit IS.mem_1; et. i; clarify. *)
+    + i. eapply used_closed; et.
+  - unfold tge. i.
+    exploit Genv_map_defs_def; et. i; des.
+    uo. des_ifs. bsimpl.
+    exploit SIMDEFINV; et. i; des. clarify. psimpl. clear_tac.
+    exploit Genv.invert_find_symbol; et. intro SYMBTGT; des.
+    exploit SIMSYMB3; et. i; des.
+    exploit Genv.find_invert_symbol; et. intro SYMBSRC.
+
+    assert(used_set tprog i).
+    { hexploit (match_prog_def _ _ _ TRANSL1 i); et. i. des_ifs. }
+
+    exploit SIMSYMB2; et.
+    { unfold used_set in *. clear - H1. des_sumbool.
+      ii. des. align_bool; bsimpl. des_sumbool. ss. des; clarify.
+      unfold defs in *. des_sumbool. ss.
+    }
+    i; des.
+    clarify. clear_tac.
+
+    assert(blk_src = b).
+    { eapply DISJ; et. }
+    clarify.
+
+    unfold ge.
+    unfold SkEnv.revive.
+    erewrite Genv_map_defs_def_inv; et.
+    uo.
+    des_ifs_safe.
+
+    hexploit (match_prog_def _ _ _ TRANSL1 i); et. intro DEFMAP. des_ifs_safe. unfold option_map in *.
+    des_ifs_safe.
+    esplits; et.
+  - eauto.
+Qed.
+
+
+Let SEGESRC: senv_genv_compat skenv_link_src ge. Proof. eapply SkEnv.senv_genv_compat; et. Qed.
+Let SEGETGT: senv_genv_compat skenv_link_tgt tge. Proof. eapply SkEnv.senv_genv_compat; et. Qed.
+
+Theorem sim_modsem
+  :
+    ModSemPair.sim msp
+.
+Proof.
+  (* rr in TRANSL. destruct TRANSL as [TRANSL0 TRANSL1]. *)
+  destruct TRANSL as [used0 TRANSL0]. des.
+  eapply match_states_sim with (match_states := match_states)
+                               (match_states_at := fun _ _ => eq)
+                               (sound_state := SoundTop.sound_state);
+    eauto; ii; ss.
+  - instantiate (1:= Nat.lt). apply lt_wf.
+  - eapply SoundTop.sound_state_local_preservation.
+  - (* init bsim *)
+    (* destruct sm_arg; ss. clarify. *)
+    destruct args_src, args_tgt; ss.
+    inv SIMARGS; ss. clarify.
+    inv INITTGT. ss.
+    assert(SIMGE: meminj_preserves_globals prog tprog (used_set tprog) ge tge (SimMemInjInv.inj sm_arg)).
+    { eapply sim_skenv_meminj_preserves_globals; et. apply SIMSKENV. }
+    des.
+    esplits; eauto.
+    + refl.
+    + econs; eauto; ss; cycle 1.
+      { inv SAFESRC. ss. }
+      * inv TYP.
+        inv SAFESRC. folder. ss.
+
+
+        inv TYP.
+        exploit find_funct_inject; et. i; des. clarify.
+        rpapply match_states_call; ss; eauto.
+        { econs; ss; et.
+          - inv SIMSKENV. ss. eapply SimSymbDropInv.sim_skenv_symbols_inject; et.
+          - inv SIMSKENV. inv MWF. inv SIMSKELINK. ss.
+          - inv SIMSKENV. inv MWF. inv SIMSKELINK. ss.
+        }
+        { eapply inject_list_typify_list; eauto. }
+        { eapply MWF. }
+  - des. inv SAFESRC.
+    inv SIMARGS; ss.
+    assert(SIMGE: meminj_preserves_globals prog tprog (used_set tprog) ge tge (SimMemInjInv.inj sm_arg)).
+    { eapply sim_skenv_meminj_preserves_globals; et. apply SIMSKENV. }
+    exploit find_funct_inject; et. i; des. clarify.
+    inv TYP.
+    esplits; eauto. econs; eauto.
+    + (* TODO: add lemma *)
+      econs; et.
+      etrans; try apply LEN; et. symmetry. eapply inject_list_length; et.
+    + etrans; try apply LEN; et. symmetry. eapply inject_list_length; et.
+  - (* call wf *)
+    inv MATCH; ss. inv MATCHST; ss.
+  - (* call fsim *)
+    des. clear_tac.
+    assert(SIMGE: meminj_preserves_globals prog tprog (used_set tprog) ge tge (SimMemInjInv.inj sm0)).
+    { eapply sim_skenv_meminj_preserves_globals; et. apply SIMSKENV. }
+    inv MATCH; ss.
+    inv CALLSRC. inv MATCHST; ss. clarify.
+    folder.
+    inv MCOMPAT; ss. clear_tac.
+    inv FPTR; try (by des; ss).
+    ss. destruct (Ptrofs.eq_dec ofs1 Ptrofs.zero); clarify; try (by des; ss).
+    esplits; try refl; eauto.
+    + econs; eauto.
+      * folder.
+        ss. des_ifs_safe.
+        inv SIMGE. uge0. des_ifs_safe. exploit defs_rev_inject; eauto. i; des. clarify. des_ifs_safe. des_ifs.
+      * clear EXTERNAL. des. ss. uge0. des_ifs_safe.
+        psimpl.
+        inv SIMSKENV. inv SIMSKELINK. ss.
+        exploit SIMDEF; et. i; des. clarify. des_ifs. esplits; et.
+    + econs; ss; et.
+  - (* after fsim *)
+    des. clear_tac.
+    assert(SIMGE: meminj_preserves_globals prog tprog (used_set tprog) ge tge (SimMemInjInv.inj sm0)).
+    { eapply sim_skenv_meminj_preserves_globals; et. apply SIMSKENV. }
+    inv AFTERSRC.
+    inv SIMRET. ss. exists sm_ret.
+    inv MATCH; ss. inv MATCHST; ss.
+    inv HISTORY. ss. clear_tac.
+    esplits; try refl; eauto.
+    + econs; eauto.
+    + econs; ss; eauto. destruct retv_src, retv_tgt; ss. clarify.
+      inv MLE0; ss.
+      inv MCOMPAT. clear_tac.
+      rpapply match_states_return; ss; eauto; ss.
+      {
+        eapply match_stacks_bound; et; cycle 1.
+        eapply match_stacks_incr; et.
+        { i. exploit FROZEN; eauto. i; des. unfold Mem.valid_block in *. esplits; eauto with xomega. }
+      }
+      { eapply inject_typify; et. }
+      { eapply MWF. }
+
+  - (* final fsim *)
+    inv MATCH. inv FINALSRC; inv MATCHST; ss.
+    inv STACKS. inv MCOMPAT; ss.
+    eexists sm0. esplits; ss; eauto. refl.
+  - (* step *)
+    left; i.
+    assert(SIMGE: meminj_preserves_globals prog tprog (used_set tprog) ge tge (SimMemInjInv.inj sm0)).
+    { eapply sim_skenv_meminj_preserves_globals; et. apply SIMSKENV. }
+
+    esplits; eauto.
+    { apply modsem_receptive; et. }
+    inv MATCH.
+    ii. hexploit (@step_simulation prog tprog (used_set tprog) skenv_link_src skenv_link_tgt); eauto.
+    i; des.
+    esplits; eauto.
+    + left. apply plus_one. econs; eauto. eapply modsem2_determinate; eauto.
+    + econs; ss.
+      * inv H0; ss; inv MCOMPAT; ss.
+      * inv H0; ss; inv MCOMPAT; ss.
+Unshelve.
+  all: ss; try (by econs).
+Qed.
+
+End SIMMODSEM.
+
+
+Section SIMMOD.
+
+Variable prog: RTL.program.
+Variable tprog: RTL.program.
+Hypothesis TRANSL: match_prog prog tprog.
+
+Definition mp: ModPair.t :=
+  ModPair.mk (RTLC.module prog) (RTLC.module tprog) ((prog.(defs) -1 tprog.(defs) -1 (Pos.eq_dec tprog.(prog_main))): ident -> Prop)
+.
+
+Theorem sim_mod
+  :
+    ModPair.sim mp
+.
+Proof.
+  econs; ss.
+  - destruct TRANSL as [used0 TRANSL0]. desH TRANSL0. clarify.
+    econs; ss.
+    + i. ss. inv TRANSL1.
+      specialize (match_prog_def id).
+      generalize (Sk.of_program_prog_defmap prog fn_sig id). intro REL0.
+      generalize (Sk.of_program_prog_defmap tprog fn_sig id). intro REL1.
+
+      destruct (classic (defs prog id)); cycle 1.
+      {
+        rewrite <- (Sk.of_program_defs fn_sig) in H.
+        inv REL0; align_opt; cycle 1.
+        { exploit prog_defmap_image; et. i; des. unfold defs in *. align_bool; bsimpl. align_bool. des_sumbool. ss. }
+        unfold fundef in *.
+        rewrite H1 in *.
+        inv REL1; align_opt; ss; clarify.
+        des_ifs.
+      }
+
+      assert(KEPT0: defs tprog id \/ Pos.eq_dec (prog_main tprog) id).
+      { tauto. }
+      clear KEPT.
+
+      assert(IN: used_set tprog id).
+      { unfold used_set. des_sumbool. ss. des; et; bsimpl.
+        - right. unfold defs in *. des_sumbool. ss.
+        - des_sumbool. clarify. tauto.
+      }
+
+      des_ifs.
+      unfold fundef in *. rewrite match_prog_def in *.
+      unfold option_map in *. des_ifs; cycle 1.
+      { unfold defs in *. des_sumbool. apply prog_defmap_spec in H. des; clarify. }
+      inv REL1. inv REL0.
+      destruct g; ss.
+      * destruct f; ss.
+        { inv H2; ss. des_ifs. inv H4; ss. des_ifs. }
+        { inv H2; ss. des_ifs. inv H4; ss. des_ifs. des_sumbool. clarify. }
+      * { inv H2; ss. des_ifs. inv H4; ss. des_ifs. inv H5; inv H2; ss. repeat f_equal. destruct i2, i3; ss. }
+
+    + i. ss. inv TRANSL1.
+      specialize (match_prog_def id).
+      generalize (Sk.of_program_prog_defmap prog fn_sig id). intro REL0.
+      generalize (Sk.of_program_prog_defmap tprog fn_sig id). intro REL1.
+
+      des. align_bool; bsimpl. align_bool. des_sumbool.
+      inv REL1; ss; align_opt.
+      rewrite <- (Sk.of_program_defs fn_sig) in DROP1.
+      exploit prog_defmap_image; et. i; des. unfold defs in *; ss. des_sumbool. ss.
+
+    + ii. unfold privs. bsimpl. des. bsimpl. des_sumbool.
+      rewrite (Sk.of_program_defs fn_sig). split; ss.
+      unfold NW. align_bool; bsimpl. des_sumbool.
+      ii.
+
+      exploit used_public; et. intro IN. unfold used_set in IN. des_sumbool. ss. des; clarify; ss.
+      unfold defs in *. des_sumbool. ss.
+
+    + inv TRANSL1; ss.
+
+    + inv TRANSL1; ss.
+    + ii. des.
+      inv TRANSL0.
+      assert(PROG0: (prog_defmap tprog) ! id = Some (Gvar gv)).
+      {
+        (* TODO: make lemma!!!!!!!!!!!!!!!!!!! *)
+        generalize (Sk.of_program_prog_defmap tprog fn_sig id). intro REL.
+        inv REL; try congruence.
+        rewrite PROG in *. clarify.
+        inv H2. inv H4. ss. destruct i1, i2; ss.
+      }
+      inv TRANSL1.
+      rewrite match_prog_def in *. des_ifs.
+      unfold option_map in PROG0. des_ifs. unfold map_globdef in H1. des_ifs.
+      exploit (used_closed id); et. ii.
+      exploit used_defined; et. i; des.
+      { exploit prog_defmap_dom; et. i; des. specialize (match_prog_def id_drop). des_ifs. rewrite H2 in *.
+        unfold defs in DROP1. apply DROP1. des_sumbool. eapply prog_defmap_image; et.
+      }
+      { clarify. apply DROP0. des_sumbool. ss. }
+    + inv TRANSL1. eapply NoDup_norepet; et. rewrite Sk.of_program_defs_names; ss.
+    + ii. des. eapply H0. des_sumbool. inv TRANSL1. eauto.
+  - ii. eapply sim_modsem; eauto.
+Unshelve.
+  all: ss.
+Qed.
+
+End SIMMOD.
+
